experiments: constructing calls to `applyRewriteCorrect`

theorems/experiments/denote_IR_3.lean
@@ -12,7 +12,7 @@ inductive IR : Nat → Type where
 
   | add (lhs rhs : IR idx) : IR idx
   | addNsw (lhs rhs : IR idx) : IR idx
-deriving BEq, Repr
+deriving BEq, Repr, ToExpr
 
 deriving instance BEq for iN
 
@@ -63,15 +63,15 @@ For the implementation to optimise, it needs to know whether or not the width as
 structure Rule where
   valid : WidthAssignment → Bool
 
-  impl : (ξ : WidthAssignment) → valid ξ → {idx : Nat} → IR idx → IR idx
+  impl : {idx : Nat} → IR idx → IR idx
 
-  wf : ∀ (ξ : WidthAssignment) (h : valid ξ) (σ : Assignment) {idx : Nat} (lhs : IR idx),
-    let rhs := impl ξ h lhs
+  wf : ∀ (ξ : WidthAssignment) (ξvalid : valid ξ) (σ : Assignment) {idx : Nat} (lhs : IR idx),
+    let rhs := impl lhs
     (IR.eval ξ σ lhs) ~> (IR.eval ξ σ rhs)
 
 def add_zero' : Rule :=
   { valid := fun ξ => true
-  , impl := fun ξ _ _ ir => match ir with
+  , impl := fun ir => match ir with
       | IR.add lhs (IR.const 0) => lhs
       | _ => ir
   , wf := by
@@ -81,21 +81,21 @@ def add_zero' : Rule :=
       apply add_zero
   }
 
-def applyRewrite {idx} (ir : IR idx) (r : Rule) (ξ : WidthAssignment) (ξvalid : r.valid ξ) : IR idx :=
-  r.impl ξ ξvalid ir
+def applyRewrite {idx} (ir : IR idx) (r : Rule) : IR idx :=
+  r.impl ir
 
 theorem applyRewriteCorrect (ir : IR idx) (r : Rule)
   (σ : Assignment) (ξ : WidthAssignment) (ξvalid : r.valid ξ)
-  : (IR.eval ξ σ ir) ~> (IR.eval ξ σ (applyRewrite ir r ξ ξvalid)) := r.wf ξ ξvalid σ ir
+  : (IR.eval ξ σ ir) ~> (IR.eval ξ σ (applyRewrite ir r)) := r.wf ξ ξvalid σ ir
 
 def A : IR 0 := IR.add (IR.var 0) (IR.const 0)
-def B {n : Nat} : IR 0 := applyRewrite A add_zero' (Lean.RArray.leaf n) (by trivial)
+def B : IR 0 := applyRewrite A add_zero'
 
 def Aeval {n} : iN n → iN n :=
   fun x => IR.eval (Lean.RArray.leaf n) (Lean.RArray.leaf ⟨x⟩) A
 
 def Beval {n} : iN n → iN n :=
-  fun x => IR.eval (Lean.RArray.leaf n) (Lean.RArray.leaf ⟨x⟩) (@B n)
+  fun x => IR.eval (Lean.RArray.leaf n) (Lean.RArray.leaf ⟨x⟩) B
 
 theorem Aeval_rewrite_Beval {n} (x : iN n) :
   Aeval x ~> Beval x :=
@@ -114,7 +114,7 @@ theorem addNsw_refine_add {n} (x y : iN n) : x +nsw y ~> x + y := by
 
 def addNsw_refine_add' : Rule :=
   { valid := fun ξ => true
-  , impl := fun ξ _ _ ir => match ir with
+  , impl := fun ir => match ir with
       | IR.addNsw lhs rhs => IR.add lhs rhs
       | _ => ir
 
@@ -130,11 +130,11 @@ def Cσ (x y : iN n) : Assignment :=
 
 /- program C is optimised into program D -/
 def C : IR 0 := IR.addNsw (IR.var 0) (IR.var 1)
-def D {n : Nat} : IR 0 := applyRewrite C addNsw_refine_add' (.leaf n) (by trivial)
+def D : IR 0 := applyRewrite C addNsw_refine_add'
 
 /- Ceval is the actual denoted semantics behind C, same for Deval -/
 def Ceval {n} (x y : iN n) : iN n := IR.eval (.leaf n) (Cσ x y) C
-def Deval {n} (x y : iN n) : iN n := IR.eval (.leaf n) (Cσ x y) (@D n)
+def Deval {n} (x y : iN n) : iN n := IR.eval (.leaf n) (Cσ x y) D
 
 /- correctness proof -/
 theorem Ceval_rewrite_Deval {n} (x y : iN n) :
@@ -144,3 +144,165 @@ theorem Ceval_rewrite_Deval {n} (x y : iN n) :
 /- but, behaviour is not equal! the behaviour of C is "refined" into D -/
 #eval @Ceval 32 (bitvec 2147483647) (bitvec 1) /- iN.poison -/
 #eval @Deval 32 (bitvec 2147483647) (bitvec 1) /- iN.bitvec 0x80000000#32 -/
+
+/- ----------------------------------------------------------------- -/
+
+partial def reifyIRExpr (idx : Nat) (assignment : Array (FVarId × Nat)) (body : Expr) : MetaM (IR idx) := do
+  match_expr body with
+  | iN.poison _ => return IR.const_poison
+  | iN.bitvec _ e =>
+    if let some (v, _) := (← getOfNatValue? e ``BitVec) then
+      return IR.const v
+
+    throwError "reifyIRExpr: unsupported bitvec expression {body}"
+
+  | iN.add _ lhs rhs =>
+    let lhs_ir ← reifyIRExpr idx assignment lhs
+    let rhs_ir ← reifyIRExpr idx assignment rhs
+    return IR.add lhs_ir rhs_ir
+  | iN.addNsw _ lhs rhs =>
+    let lhs_ir ← reifyIRExpr idx assignment lhs
+    let rhs_ir ← reifyIRExpr idx assignment rhs
+    return IR.addNsw lhs_ir rhs_ir
+  | _ =>
+
+    if let some fvarid := body.fvarId? then
+      let some varIdx := assignment.findIdx? (fun (fid, _) => fid == fvarid)
+        | throwError "reifyIRExpr: unbound free variable {body}"
+
+      return IR.var varIdx
+
+    throwError "reifyIRExpr: unsupported expression {body}"
+
+structure PackedIR where
+  {idx : Nat}
+  ir : IR idx
+deriving Repr
+
+def reifyExprApply (rule : Rule) (ruleExpr : Q(Rule)) (e : Expr) : MetaM PackedIR := do
+  /- doesn't support hypotheses such as `fun {n} {m} (h : m ≤ n) (x : iN n) : iN m := ...`,
+    hence valid is just set to returning true always -/
+
+  lambdaTelescope e fun fvars body => do
+
+    /- map each type iN n -> idx of WidthAssignment -/
+    /- these are fvars being m, n, ... -/
+    let mut width_assignment : Array FVarId := #[]
+
+    /- map each expr x -> idx of Assignment -/
+    let mut assignment : Array (FVarId × Nat) := #[]
+
+    for fvar in fvars do
+      /- https://github.com/leanprover-community/quote4/issues/36 -/
+      let fvar_type ← inferType fvar
+
+      match_expr fvar_type with
+      | Nat =>
+        width_assignment := width_assignment.push fvar.fvarId!
+      | iN nv =>
+
+        /- n should be an fvar, if we have for example (x : iN 32),
+          we should encode it as ∀n : Nat, n = 32 → ... inside valid.
+          this is unhandled for now -/
+        let some assignmentIdx := width_assignment.findIdx? (fun widthFvar => widthFvar == nv.fvarId!)
+          | throwError "reifyExpr: unbound, not previous free variable in Nat"
+
+        assignment := assignment.push (fvar.fvarId!, assignmentIdx)
+      | _ => throwError "reifyExpr: unsupported type"
+
+    if h : ¬0 < assignment.size then
+      unreachable!
+    else if h' : ¬0 < width_assignment.size then
+      unreachable!
+    else
+
+    let body_type ← inferType body
+    let resultIdx ← match_expr body_type with
+    | iN nv =>
+
+      let some assignmentIdx := width_assignment.findIdx? (fun widthFvar => widthFvar == nv.fvarId!)
+        | throwError "reifyExpr: unbound, not previous free variable in Nat"
+
+      pure assignmentIdx
+    | _ => throwError "reifyExpr: unsupported body type {body_type}"
+
+    let ir ← reifyIRExpr resultIdx assignment body
+
+    have resultIdxQ : Q(Nat) := toExpr resultIdx
+    have irQ : Q(IR $resultIdxQ) := toExpr ir
+
+    let assignment' : RArray (FVarId × Nat) :=
+      RArray.ofArray assignment (by exact Decidable.of_not_not h)
+
+    let width_assignment' : RArray FVarId :=
+      RArray.ofArray width_assignment (by exact Decidable.of_not_not h')
+
+    have ξQ : Q(WidthAssignment) :=
+      ← width_assignment'.toExpr q(Nat) fun (fvar : FVarId) => mkFVarEx fvar
+
+    have σQ : Q(Assignment) :=
+      ← assignment'.toExpr q(PackediN) fun (⟨x, idx⟩ : FVarId × Nat) =>
+        /- we want iN (ξ.get idx) -/
+        /- ⟨ξ.get idx, x⟩ -/
+
+        have idxQ : Q(Nat) := toExpr idx
+
+        have xQ : Q(iN (($ξQ).get $idxQ)) := mkFVarEx x
+        have fid : Q(PackediN) := q(@PackediN.mk (($ξQ).get $idxQ) $xQ)
+        fid
+
+    let proof := q(@applyRewriteCorrect $resultIdxQ $irQ $ruleExpr $σQ $ξQ sorry)
+    check proof
+
+    logInfo m!"proof: {proof}"
+    let proofType ← inferType proof
+
+    match_expr proofType with
+    | Rewrite _ lhs rhs =>
+      logInfo m!"lhs: {← reduceAll lhs}"
+      logInfo m!"rhs: {← reduceAll rhs}"
+    | _ => pure ()
+
+    /- let ⟨_, ~q(Rewrite $n $lhs $rhs), ~q($e)⟩ ← inferTypeQ proof | throwError "reifyExprApply: unexpected proof type"
+ -/
+    logInfo m!"proofType: {proofType}"
+
+    /- let proofReduced ← reduce proofType
+    logInfo m!"proofTypeReduced: {proofReduced}" -/
+
+
+    return ⟨rule.impl ir⟩
+
+unsafe def evalPleaseImpl (expr : Expr) : MetaM Rule :=
+  evalExpr Rule q(Rule) expr
+
+@[implemented_by evalPleaseImpl]
+opaque evalPlease (expr : Expr) : MetaM Rule
+
+syntax rwRuleSeq := "[" withoutPosition(term,*,?) "]"
+
+/- accepts expressions of the form
+  `fun {n} ... {m} (x : iN n) ... (z : iN m) : iN n => ...` -/
+elab "⟪" t:term "⟫" s:rwRuleSeq : term => do
+  let t ← Term.elabTerm t none
+
+  match s with
+  | `(rwRuleSeq| [$rs,*]) =>
+    let rewrites ← Term.withoutErrToSorry do
+      let rewrites ← rs.getElems.mapM fun te => Term.elabTermEnsuringType te q(Rule)
+      MetaM.run' (rewrites.mapM evalPlease)
+
+    logInfo m!"rewrites: {rewrites.size}"
+
+    /- TODO handle other rewrites -/
+    let irExpr ← reifyExprApply addNsw_refine_add' q(addNsw_refine_add') t
+    logInfo m!"reified IR: {repr irExpr}"
+
+    return t
+  | _ => throwUnsupportedSyntax
+
+
+--#eval ⟪fun {n} {m} (x : iN n) (y : iN m) => y⟫
+def fn := ⟪fun {n} (x : iN n) => x +nsw x⟫ []
+
+#print fn
